ImpE2.v
@@ -445,7 +445,12 @@ Section Semantics.
 End Semantics.
   
 Section Preservation.
-
+  Parameter S : set condition.
+  Parameter U : set condition.
+  Parameter g: sec_spec.
+  Definition cnd_in_S (l: location) (m0 : mem2) : Prop :=
+    is_Cnd l /\ m0 l = VSingle (Vnat 1).
+  
   Ltac unfold_cfgs :=
     unfold ccfg_update_reg2 in *;
     unfold ccfg_to_ecfg2 in *;
@@ -455,26 +460,24 @@ Section Preservation.
     unfold ccfg_com2 in *;
     unfold ecfg_exp2 in *;
     unfold ecfg_reg2 in *;
-    unfold ecfg_update_exp2 in *.                      
+    unfold ecfg_update_exp2 in *.                   
 
-  Definition cterm2_ok (G: context) (d: loc_mode) (S: set condition) (H: set esc_hatch)
-             (m0: mem2) (r: reg2) (m: mem2) (K: kill2) : Prop :=
+  Definition cterm2_ok (G: context) (d: loc_mode) (m0: mem2)
+             (r: reg2) (m: mem2) (K: kill2) : Prop :=
       (forall x v1 v2 bt p,
           (r x = VPair v1 v2 /\ (var_context G) x = Some (Typ bt p)) -> protected p S) 
       /\ (forall l v1 v2 bt p rt,
           (m (Not_cnd l) = VPair v1 v2 /\ (loc_context G) (Not_cnd l) = Some (Typ bt p, rt))
           -> protected p S)
-      /\ (forall e v md', set_In e H ->
-                          is_esc_hatch e ->
+      /\ (forall e v md', is_esc_hatch e G ->
                           (estep2 md' d (e, reg_init2, m0, K) v ->
                            estep2 md' d (e, r, m, K) v))
-      /\ project_kill K true = project_kill K false.
+      /\ project_kill K true = project_kill K false
+      /\ knowledge_ind (project_mem m0 true) g U L (project_mem m0 false).
 
   Definition cconfig2_ok (pc: sec_policy) (md: mode) (G: context) (U: set condition)
-             (d: loc_mode) (S: set condition) (H: set esc_hatch) (m0: mem2)
-             (ccfg2: cconfig2) (G': context) (K': kill2) : Prop :=
+             (d: loc_mode) (m0: mem2) (ccfg2: cconfig2) (G': context) (K': kill2) : Prop :=
     (forall i, set_In i U -> (ccfg_mem2 ccfg2) (Cnd i) = VSingle (Vnat 0))
-    (* unsure about this kill set thing.. pretty sure we can assume this from lemma 3 *)
     /\  com_type pc md G (project_kill (ccfg_kill2 ccfg2) true) U d
                  (ccfg_com2 ccfg2) G' (project_kill K' true)
     /\ (forall x v1 v2 bt p,
@@ -485,15 +488,15 @@ Section Preservation.
            ((ccfg_mem2 ccfg2) (Not_cnd l) = VPair v1 v2
             /\ (loc_context G) (Not_cnd l) = Some (Typ bt p, rt))    
            -> protected p S)
-    /\ (forall e v md', set_In e H ->
-                        is_esc_hatch e ->
+    /\ (forall e v md', is_esc_hatch e G ->
                         (estep2 md' d  (e, reg_init2, m0, ccfg_kill2 ccfg2) v ->
                          estep2 md' d (e, ccfg_reg2 ccfg2, ccfg_mem2 ccfg2, ccfg_kill2 ccfg2) v))
-    /\ project_kill (ccfg_kill2 ccfg2) true = project_kill (ccfg_kill2 ccfg2) false.
+    /\ project_kill (ccfg_kill2 ccfg2) true = project_kill (ccfg_kill2 ccfg2) false
+    /\ knowledge_ind (project_mem m0 true) g U L (project_mem m0 false).
 
   Lemma esc_hatch_reg_irrelevance (e : esc_hatch) :
-    forall md d r m k v r',
-    is_esc_hatch e -> estep2 md d (e, r, m, k) v ->
+    forall G md d r m k v r',
+    is_esc_hatch e G -> estep2 md d (e, r, m, k) v ->
     estep2 md d (e, r', m, k) v.
   Proof.
     intros. unfold is_esc_hatch in *.
@@ -502,22 +505,39 @@ Section Preservation.
     induction H0; intros; subst; auto.
     1-3: constructor; unfold_cfgs; auto.
     - unfold_cfgs. subst. unfold exp_novars in H1. simpl in H1. omega.
-    - unfold_cfgs; subst.
-      assert (exp_novars e1 /\ exp_novars e2). unfold exp_novars in *;
-                                                 inversion H0; destruct_pairs; auto.
-      destruct_pairs.
-      pose (IHestep2_1 e1 H). pose (IHestep2_2 e2 H1).
+    - unfold_cfgs; subst; destruct_pairs.
+      assert (exp_novars e1 /\ all_loc_immutable e1 G).
+      split. unfold exp_novars in *. destruct_pairs; inversion H; destruct_pairs; auto.
+      unfold all_loc_immutable in *; destruct_pairs; inversion H0; destruct_pairs; auto.
+      assert (exp_novars e2 /\ all_loc_immutable e2 G).
+      split. unfold exp_novars in *. destruct_pairs; inversion H; destruct_pairs; auto.
+      unfold all_loc_immutable in *; destruct_pairs; inversion H0; destruct_pairs; auto.
+      pose (IHestep2_1 e1 H1); pose (IHestep2_2 e2 H2).
       apply (Estep2_binop md d (Ebinop e1 e2 op,r',m,k) e1 e2 n1 n2); unfold_cfgs; auto.
-    - inversion Heqecfg2; subst.
-      assert (exp_novars e). unfold exp_novars in *. inversion H3; auto.
+    - inversion Heqecfg2; subst; destruct_pairs.
+      assert (exp_novars e). unfold exp_novars in *; destruct_pairs; inversion H; auto.
       apply (Estep2_deref md d (Ederef e,r',m,k) e r' m k l (m l)); unfold_cfgs; auto.
-    - unfold_cfgs. subst.
-      apply (Estep2_isunset md d (Eisunset cnd,r',m,k) cnd v); unfold_cfgs; auto.
-      assert (exp_novars (Ederef (Eloc (Cnd cnd)))). unfold exp_novars. simpl; auto.
-      apply IHestep2 in H; auto.
+      apply (IHestep2 e); split; auto.
+      unfold all_loc_immutable in *; inversion H1; auto.
+    - unfold_cfgs; subst.
+      destruct_pairs. unfold all_loc_immutable in H2. simpl in H2. omega.
   Qed.
 
-  Lemma econfig2_pair_protected : forall md G d e p r m k v v1 v2 S bt H m0,
+  (*Lemma esc_hatch_nopairs_equivalent (e : esc_hatch) : *)
+
+  Lemma econfig2_locs_protected (e: exp) (m0: mem2):
+    forall G d r m k v v1 v2 bt bt' p p' q md md' rt e',
+      knowledge_ind (project_mem m0 true) g U L (project_mem m0 false) ->
+      v = VPair v1 v2 ->
+      exp_type md G d e (Typ bt p) ->
+      estep2 md d (e,r,m,k) v ->
+      e = Ederef e' ->
+      exp_type md G d e' (Typ (Tref (Typ bt' p') md' rt) q) ->
+      protected p S.
+  Proof.
+  Admitted.
+
+  Lemma econfig2_pair_protected : forall md G d e p r m k v v1 v2 bt m0,
       v = VPair v1 v2 ->
       exp_type md G d e (Typ bt p) ->
       estep2 md d (e,r,m,k) v ->
@@ -528,42 +548,42 @@ Section Preservation.
           e = Ederef e' ->
           exp_type md G d e' (Typ (Tref (Typ bt' p') md' rt) q)
           -> protected q S) ->
-      cterm2_ok G d S H m0 r m k ->
+      cterm2_ok G d m0 r m k ->
       protected p S.
   Proof.
     intros.
     remember (e,r,m,k) as ecfg.
     generalize dependent e.
-    induction H2; intros; subst; try discriminate; unfold_cfgs;
-    unfold cterm2_ok in H4; destruct_pairs; subst.
-    - inversion H3; subst.
-      apply (H0 x v1 v2 bt p); split; auto. 
+    induction H1; intros; subst; try discriminate; unfold_cfgs;
+    unfold cterm2_ok in H3; destruct_pairs; subst.
+    - inversion H2; subst.
+      apply (H x v1 v2 bt p); split; auto. 
     - inversion Heqecfg; subst.
-      inversion H6; subst.
-      assert (protected q S). apply (H7 bt p0 q md' rt e); auto.
+      inversion H5; subst.
+      assert (protected q S). apply (H6 bt p0 q md' rt e); auto.
       apply (join_protected_r S p0 q); auto.
-    - destruct H3; destruct_pairs; try discriminate.
+    - destruct H2; destruct_pairs; try discriminate.
   Qed.
 
-  Lemma impe2_final_config_preservation 
-        (G: context) (d: loc_mode) (S: set condition) (H: set esc_hatch) (m0: mem2) :
+  Lemma impe2_final_config_preservation (G: context) (d: loc_mode) (m0: mem2) :
       forall G' K' c r m k pc md U r' m' t,
         (forall l e v, loc_in_exp e G l -> m0 l = VSingle v) -> 
         context_wt G d ->
-        cconfig2_ok pc md G U d S H m0 (c,r,m,k) G' K' ->
+        cconfig2_ok pc md G U d m0 (c,r,m,k) G' K' ->
         cstep2 md d (c,r,m,k) (r', m', K') t ->
-        cterm2_ok G' d S H m0 r' m' K'.
+        cterm2_ok G' d m0 r' m' K'.
   Proof.
-    intros; remember (c,r,m,k) as ccfg2; subst.
-    unfold cconfig2_ok in H2; destruct_pairs.
+    intros G' K' c r m k pc md U r' m' t Hlocs Hcwt Hcfgok Hcstep.
+    remember (c,r,m,k) as ccfg2; subst.
+    unfold cconfig2_ok in Hcfgok; destruct_pairs.
     induction c; unfold cterm2_ok; intros; subst; simpl in *; unfold_cfgs.
     (* CSkip *)
-    - inversion H3; try discriminate; subst;
-        inversion H4; try discriminate; subst.
+    - inversion Hcstep; try discriminate; subst.
+        inversion H0; try discriminate; subst.
       split; [intros | split; intros]; simpl in *; auto.
-      -- now apply H5 in H10.
-      -- now apply H6 in H10.
-    (* CAssign *)
+      -- now apply H1 in H7.
+      -- now apply H2 in H7.
+(*    (* CAssign *)
     - inversion H3; try discriminate; subst;
         inversion H4; try discriminate; subst.
       split; [intros | split; intros]; simpl in *; auto; unfold_cfgs.
@@ -599,13 +619,14 @@ Section Preservation.
       --- rewrite <- (Nat.eqb_eq x0 x) in e; rewrite e in *.
           
           inversion H11; try discriminate; subst.
+*)
   Admitted.
          
   Lemma impe2_type_preservation
         (G: context) (d: loc_mode) (S: set condition) (H: set esc_hatch) (m0: mem2) :
     forall pc md U c r m K G' K',
       context_wt G d ->
-      cconfig2_ok pc md G U d S H m0 (c, r, m, K) G' K' ->
+      cconfig2_ok pc md G U d m0 (c, r, m, K) G' K' ->
       forall mdmid cmid rmid mmid rmid' mmid' kmid' tmid rfin mfin kfin tfin,
         imm_premise
           (cstep2 mdmid d (cmid, rmid, mmid, K') (rmid', mmid', kmid') tmid)
@@ -613,7 +634,7 @@ Section Preservation.
         (exists pcmid Gmid Gmid' Umid,
           policy_le pc pcmid ->
           Umid = [] \/ (forall i, In i U -> In i Umid) ->
-          cconfig2_ok pcmid mdmid Gmid Umid d S H m0 (cmid, rmid, mmid, K') Gmid' K').
+          cconfig2_ok pcmid mdmid Gmid Umid d m0 (cmid, rmid, mmid, K') Gmid' K').
   Proof.
   Admitted.
  
@@ -825,7 +846,7 @@ Section Adequacy.
       admit.
      (* XXX: I think there's a typo in the paper's While-div rule that I need to figure out *)
      (* destruct is_left; [destruct n1 | destruct n2]; rewrite project_merge_inv_trace.
-      +  assert (t1 = [] /\ k1 = (project_kill K true) /\
+      +  assert (t1 = [] /\ k1 = (project_kill xK true) /\
                  (project_reg r true) = (project_reg r' true) /\
                  (project_mem m true) = (project_mem m' true)) by
             (inversion H1; subst; auto; try discriminate); destruct_conjs; subst.
